Nerodia/Data/PyInt/Basic.lean
@@ -1,0 +1,90 @@
+/-
+Copyright (c) 2026 Lean FRO. All rights reserved.
+Released under Apache 2.0 license as described in the file LICENSE.
+Authors: Mac Malone
+-/
+module
+public import Nerodia.Data.Types
+public import Nerodia.Data.OfPyArg
+public import Nerodia.Data.MkResult
+public import Nerodia.Data.PyStr.Basic
+public import Nerodia.Control.CPyIO
+
+namespace Nerodia
+
+/--
+Creates a Python integer from a
+two's complement encoding in little-endian byte order.
+-/
+@[extern "nerodia_mk_py_int_le"]
+opaque mkPyIntLE (n : @& ByteArray) : CPyIO PyInt
+
+@[export nerodia_mk_big_py_int]
+partial def mkBigPyInt (n : Int) : CPyIO PyInt :=
+  mkPyIntLE (toByteArrayLE n)
+where
+  @[inline] toByteArrayLE (n : Int) : ByteArray :=
+    let bs := ByteArray.emptyWithCapacity 32
+    loop (bs.push n.toInt8.toUInt8) (n / 256)
+  loop bs n :=
+    let n' := n / 256
+    if n = n' then
+      bs
+    else
+      loop (bs.push n.toInt8.toUInt8) n'
+
+/-- Creates a Python integer from a Lean integer. -/
+@[extern "nerodia_mk_py_int"]
+public opaque mkPyInt (n : @& Int) : CPyIO PyInt
+
+public instance : MkCResult Int int := ⟨mkPyInt⟩
+
+namespace PyInt
+
+@[extern "nerodia_py_int_to_byte_array_le"]
+opaque toByteArrayLE' (self : @& PyInt) : {bs : ByteArray // 0 < bs.size } :=
+  ⟨.mk #[default], by simp [ByteArray.size]⟩
+
+/--
+Returns the two's-complement encoding of
+{lean}`self` in little-endian byte order.
+-/
+@[inline] public def toByteArrayLE (self : @& PyInt) : ByteArray :=
+  self.toByteArrayLE'.val
+
+public theorem size_toByteArrayLE_pos : 0 < (toByteArrayLE self).size :=
+  self.toByteArrayLE'.property
+
+@[extern "nerodia_py_int_to_byte_array_be"]
+opaque toByteArrayBE' (self : @& PyInt) : {bs : ByteArray // 0 < bs.size } :=
+  ⟨.mk #[default], by simp [ByteArray.size]⟩
+
+/--
+Returns the two's-complement encoding of
+{lean}`self` in big-endian byte order.
+-/
+@[inline] public def toByteArrayBE (self : @& PyInt) : ByteArray :=
+  self.toByteArrayBE'.val
+
+public theorem size_toByteArrayBE_pos : 0 < (toByteArrayBE self).size :=
+  self.toByteArrayBE'.property
+
+/-- Returns the numeric value of {lean}`self` as a Lean {lean}`Int`.-/
+@[inline] public def toInt (self : @& PyInt) : Int :=
+  ofByteArrayBE self.toByteArrayBE size_toByteArrayBE_pos
+where ofByteArrayBE (bs : ByteArray) (h : 0 < bs.size) := Id.run do
+  let mut n := (bs[0]'h).toInt8.toInt
+  for h : i in 1...bs.size do
+    n := n * 256 + bs[i].toNat
+  return n
+
+public instance : OfPyArg Int int where
+  ofPyArg fn i arg :=
+    if h : arg.isIntInstance then
+      return (PyInt.mk arg h).toInt
+    else raiseArgTypeMismatch fn i arg int
+
+@[inline] public protected def toString (self : PyInt) : String :=
+  toString self.toInt
+
+public instance : ToString PyInt := ⟨PyInt.toString⟩
